src/Distributions/BernoulliExpNeg/Model.dfy
@@ -10,67 +10,64 @@ module BernoulliExpNeg.Model {
   import WhileAndUntil
   import BernoulliModel = Bernoulli.Model
 
-  ghost function Sample(gamma: Rationals.Rational): Partial.Hurd<bool>
+  ghost function Sample(gamma: Rationals.Rational): Monad.Hurd<bool>
     requires gamma.denom != 0
     requires gamma.numer >= 0
   {
-    Partial.Bind(
+    Monad.Bind(
       GammaReductionLoop(true, gamma),
       (bgamma: (bool, Rationals.Rational)) =>
         if bgamma.0 then
           SampleGammaLe1(bgamma.1)
         else
-          Partial.Return(false)
+          Monad.Return(false)
     )
   }
 
-  ghost function GammaReductionLoop(b: bool, gamma: Rationals.Rational): Partial.Hurd<(bool, Rationals.Rational)>
+  ghost function GammaReductionLoop(b: bool, gamma: Rationals.Rational): Monad.Hurd<(bool, Rationals.Rational)>
     requires gamma.numer >= 0
     decreases gamma.numer
   {
     if b && gamma.denom <= gamma.numer
     then
-      Partial.Bind(
+      Monad.Bind(
         SampleGammaLe1(Rationals.Int(1)),
         b' => GammaReductionLoop(b', Rationals.Rational(gamma.numer - gamma.denom, gamma.denom))
       )
     else
-      Partial.Return((b, gamma))
+      Monad.Return((b, gamma))
   }
 
-  ghost function SampleGammaLe1(gamma: Rationals.Rational): Partial.Hurd<bool>
+  ghost function SampleGammaLe1(gamma: Rationals.Rational): Monad.Hurd<bool>
   {
     if 0 <= gamma.numer <= gamma.denom
-    then Partial.Bind(
+    then Monad.Bind(
            GammaLe1Loop(gamma, (true, 0)),
-           (ak: (bool, nat)) => Partial.Return(ak.1 % 2 == 1)
+           (ak: (bool, nat)) => Monad.Return(ak.1 % 2 == 1)
          )
-    else Partial.Return(false) // to keep this function total, we return a dummy value here
+    else Monad.Return(false) // to keep this function total, we return a dummy value here
   }
 
-  ghost function GammaLe1Loop(gamma: Rationals.Rational, ak: (bool, nat)): Partial.Hurd<(bool, nat)>
+  ghost function GammaLe1Loop(gamma: Rationals.Rational, ak: (bool, nat)): Monad.Hurd<(bool, nat)>
     requires 0 <= gamma.numer <= gamma.denom
   {
     assume {:axiom} false; // assume termination
-    Partial.Bind(
+    Monad.Bind(
       WhileAndUntil.ProbWhile(
-        (ak: Partial.Wrap<(bool, nat)>) => ak.Satisfies((x: (bool, nat)) => x.0),
-        (ak: Partial.Wrap<(bool, nat)>) =>
-          match ak
-          case Terminating(ak) => GammaLe1LoopIter(gamma, ak)
-          case Diverging => Partial.Diverge(),
-        Partial.Terminating(ak)
+        (ak: (bool, nat)) => ak.0,
+        (ak: (bool, nat)) => GammaLe1LoopIter(gamma, ak),
+        ak
       ),
-      (ak: Partial.Wrap<(bool, nat)>) => Monad.Return(ak)
+      (ak: (bool, nat)) => Monad.Return(ak)
     )
   }
 
-  ghost function GammaLe1LoopIter(gamma: Rationals.Rational, ak: (bool, nat)): Partial.Hurd<(bool, nat)>
+  ghost function GammaLe1LoopIter(gamma: Rationals.Rational, ak: (bool, nat)): Monad.Hurd<(bool, nat)>
     requires 0 <= gamma.numer <= gamma.denom
   {
-    Partial.Bind(
+    Monad.Bind(
       BernoulliModel.Sample(gamma.numer, (ak.1 + 1) * gamma.denom),
-      (a': bool) => Partial.Return((a', ak.1 + 1))
+      (a': bool) => Monad.Return((a', ak.1 + 1))
     )
   }
 }
