src/Distributions/Uniform/Model.dfy
@@ -14,10 +14,9 @@ module Uniform.Model {
   import UniformPowerOfTwo
 
   // Definition 49
-  ghost function Sample(n: nat): Partial.Hurd<nat>
+  ghost function Sample(n: nat): Monad.Hurd<nat>
     requires n > 0
   {
-    SampleTerminates(n);
     WhileAndUntil.ProbUntil(Proposal(n), Accept(n))
   }
 
@@ -33,53 +32,9 @@ module Uniform.Model {
     (m: nat) => m < n
   }
 
-  ghost function IntervalSample(a: int, b: int): (f: Partial.Hurd<int>)
+  ghost function IntervalSample(a: int, b: int): (f: Monad.Hurd<int>)
     requires a < b
   {
-    (s: RandomNumberGenerator.RNG) =>
-      var (x, s') := Sample(b - a)(s);
-      (x.Map(x => a + x), s')
-  }
-
-  lemma SampleTerminates(n: nat)
-    requires n > 0
-    ensures
-      && Independence.IsIndepFn(Proposal(n))
-      && Quantifier.ExistsStar(WhileAndUntil.ProposalIsAccepted(Proposal(n), Accept(n)))
-      && WhileAndUntil.ProbUntilTerminates(Proposal(n), Accept(n))
-  {
-    assert Independence.IsIndepFn(Proposal(n)) by {
-      UniformPowerOfTwo.Correctness.SampleIsIndepFn(2 * n);
-    }
-    var e := iset s | WhileAndUntil.ProposalIsAccepted(Proposal(n), Accept(n))(s);
-    assert e in RandomNumberGenerator.event_space by {
-      assert e == MeasureTheory.PreImage(s => UniformPowerOfTwo.Model.Sample(2 * n)(s).0, (iset m: nat | m < n));
-      assert MeasureTheory.PreImage(s => UniformPowerOfTwo.Model.Sample(2 * n)(s).0, (iset m: nat | m < n)) in RandomNumberGenerator.event_space by {
-        assert Independence.IsIndepFn(UniformPowerOfTwo.Model.Sample(2 * n)) by {
-          UniformPowerOfTwo.Correctness.SampleIsIndepFn(2 * n);
-        }
-        assert MeasureTheory.IsMeasurable(RandomNumberGenerator.event_space, MeasureTheory.natEventSpace, s => UniformPowerOfTwo.Model.Sample(2 * n)(s).0) by {
-          Independence.IsIndepFnImpliesFstMeasurableNat(UniformPowerOfTwo.Model.Sample(2 * n));
-        }
-      }
-    }
-    assert Quantifier.ExistsStar(WhileAndUntil.ProposalIsAccepted(Proposal(n), Accept(n))) by {
-      assert RandomNumberGenerator.mu(e) > 0.0 by {
-        assert e == (iset s | UniformPowerOfTwo.Model.Sample(2 * n)(s).0 < n);
-        assert n <= Helper.Power(2, Helper.Log2Floor(2 * n)) by {
-          Helper.NLtPower2Log2FloorOf2N(n);
-        }
-        calc {
-          RandomNumberGenerator.mu(e);
-        == { UniformPowerOfTwo.Correctness.UnifCorrectness2Inequality(2 * n, n); }
-          n as real / (Helper.Power(2, Helper.Log2Floor(2 * n)) as real);
-        >
-          0.0;
-        }
-      }
-    }
-    assert WhileAndUntil.ProbUntilTerminates(Proposal(n), Accept(n)) by {
-      WhileAndUntil.EnsureProbUntilTerminates(Proposal(n), Accept(n));
-    }
+    Monad.Map(x => a + x, Sample(b - a))
   }
 }
