src/Distributions/Coin/Interface.dfy
@@ -4,7 +4,7 @@
  *******************************************************************************/
 
 module Coin.Interface {
-  import Partials
+  import Monad
   import RandomNumberGenerator
   import Model
 
@@ -15,7 +15,7 @@ module Coin.Interface {
 
     method CoinSample() returns (b: bool)
       modifies this
-      ensures Model.Sample(old(s)) == Partials.Terminating((b, s))
+      ensures Model.Sample(old(s)) == Monad.Terminating(b, s)
     {
       b := ExternCoinSample();
       assume {:axiom} false; // assume correctness of extern implementation
