src/Distributions/Uniform/Interface.dfy
@@ -4,6 +4,7 @@
  *******************************************************************************/
 
 module Uniform.Interface {
+  import Monad
   import Coin
   import Model
   import UniformPowerOfTwo
@@ -15,18 +16,18 @@ module Uniform.Interface {
       decreases *
       requires n > 0
       ensures u < n
-      ensures Model.Sample(n)(old(s)) == (Partial.Terminating(u), s)
+      ensures Model.Sample(n)(old(s)) == Monad.Terminating(u, s)
 
     method UniformIntervalSample(a: int, b: int) returns (u: int)
       modifies this
       decreases *
       requires a < b
       ensures a <= u < b
-      ensures Model.IntervalSample(a, b)(old(s)) == (Partial.Terminating(u), s)
+      ensures Model.IntervalSample(a, b)(old(s)) == Monad.Terminating(u, s)
     {
       var v := UniformSample(b - a);
-      assert Model.Sample(b-a)(old(s)) == (Partial.Terminating(v), s);
-      assert Model.IntervalSample(a, b)(old(s)) == (Partial.Terminating(a + v), s);
+      assert Model.Sample(b-a)(old(s)) == Monad.Terminating(v, s);
+      assert Model.IntervalSample(a, b)(old(s)) == Monad.Terminating(a + v, s);
       u := a + v;
     }
 
